---
title: Square Root
created: 0001-05-28
modified: 2025-05-28
---
## 1.1 
1. $\sqrt[3]{1000} = 10 \cdot 10 \cdot 10 = \underline{\underline{10^3}}$
2. $\sqrt[3]{64} = 4 \cdot 4 \cdot 4 = \underline{\underline{4^3}}$
3. $\sqrt[3]{-1} = \underline{\underline{-1}}$
4. $\sqrt[5]{32} = 2 \cdot 2 \cdot 2 \cdot 2 \cdot 2 = \underline{\underline{2^5}}$
5. $\sqrt[4]{256} = 4 \cdot 4 \cdot 4 \cdot 4 = \underline{\underline{4^4}}$

## 1.2 

Sort the following square root equations from lowest number to highest number.

$$\sqrt[3]{27} \quad \sqrt[4]{16} \quad \sqrt[7]{1} \quad \sqrt{100} \quad \sqrt[4]{40} \quad \sqrt[5]{-1}$$

Solution for the question is the following.

$$\sqrt[5]{-1} \quad \sqrt[7]{1} \quad \sqrt[4]{16} \quad \sqrt[4]{40} \quad \sqrt[3]{27} \quad \sqrt{100}$$
## 1.3

Finding the nroot with 3 decimals with Geogebra CAS.

1. $\sqrt[3]{10} = 2.154^3$
2. $\sqrt[4]{17} = 3.050^4$
3. $\sqrt[7]{-64} = 1.811^7$
4. $\sqrt[12]{1,065} = 1.005^{12}$

## 1.4 

1. $\frac{x^4 \cdot x^2}{x \cdot x^3} = \frac{x^{4 + 2}}{x^{3 + 1}} = \frac{x^6}{x^4} = x^{6 - 4} = x^2$
2. $\frac{\left(5x^2\right)^2}{5x^3} = \frac{5x^{2 \cdot 2}}{5x^3} = \frac{5x^4}{5x^3} = 5x^{4 - 3} = 5x$
3. $\left(\frac{1}{x}\right)^6 \cdot \left(x^2\right)^3 = \frac{1^6}{x^6} \cdot x^{2 \cdot 3} = \frac{1}{x^6} \cdot x^6 = 1$
4. $\frac{\left(x^{-3}\right)^{-1}}{(2x)^2} = \frac{x^{-3 \cdot -1}}{\left(2x\right)^2} = \frac{x^3}{2^2x^2} = \frac{x^{3 - 2}}{2^2} = \frac{x}{2 \cdot 2} = \frac{1}{4}x$

## 1.5

1. $\frac{a^6 \cdot b^2}{a^3 \cdot b} = a^{6 - 3} \cdot b^{2-1} = a^3 \cdot b$
2. $\frac{a^3 b^9}{a^2\left(b^{-3}\right)^3 } = \frac{a^3 b^9}{a^2 b^{-3 \cdot 3}} = \frac{a^3 b^9}{a^2 b^{-9}} = a^{3 - 2} b^{9 - (-9)} = ab^{18}$
3. $\frac{\left(2a\right)^2 \cdot b^0}{ab^{-3}} = \frac{2^2a^2 \cdot b^0}{ab^{-3}} = 2^2 a^{2 - 1} \cdot b^{0 - (-3)} = 4a \cdot b^3 = 4ab^3$
4. $\frac{\left(2ab^2\right)^3}{ 2a^3 \cdot 2ab^{-1}} = \frac{2^3 a^3 b^{2 \cdot 3}}{2a^3 \cdot 2ab^{-1}} = \frac{8a^3b^6}{\left(2 \cdot 2\right) a^{3 + 1} b^{-1}} = \frac{8a^3b^6}{4a^4b^{-1}} = \left(8 \div 4\right) a^{3 - 4} b^{6 - (-1)} = 2a^{-1}b^7$

## 1.6 

1. $\left( \frac{a}{b}\right)^p = \frac{a}{b} \cdot \frac{a}{b} \dotsm \frac{a}{b} = \frac{a^p}{b^p} = b \neq 0$
2. $\frac{a^p}{a^q} = \frac{a \cdot a \dotsm a}{a \cdot a \dotsm a} = a \neq 0$

## 1.7

1. $\sqrt[3]{7} = 7^{\frac{1}{3}}$
2. $5^{\frac{1}{2}} = \sqrt{5}$
3. $\sqrt[5]{3^4} = 3^{\frac{4}{5}}$
4. $y^{\frac{3}{4}} = \sqrt[4]{y^3}$
5. $7^{\frac{1}{4}} = \sqrt[4]{7}$

## 1.8

1. $\left(\sqrt{n}\right)^2 = n^{\frac{2}{2}} = n$
2. $\sqrt[3]{y^{9}} = y^{\frac{9}{3}} = y^3$
3. $a \sqrt{a} = a^{1 + \frac{1}{2}} = a^{\frac{2}{2} + \frac{1}{2}} = a^{\frac{3}{2}}$
4. $x \cdot \sqrt[3]{x} \cdot \sqrt[3]{x^2} = x \cdot x^{\frac{1}{3}} \cdot x^{\frac{2}{3}} = x^{\frac{3}{3} + \frac{1}{3} + \frac{2}{3}} = x^{\frac{6}{3}} = x^{2}$

## 1.9 
1. $\sqrt[5]{y} \cdot \sqrt[10]{y^8} = y^{\frac{1}{5}} \cdot y^{\frac{8}{10}} = y^{\frac{1 \cdot 2}{5 \cdot 2}} \cdot y^{\frac{8}{10}} = y^{\frac{2}{10}} \cdot y^{\frac{8}{10}} = y^{\frac{2}{10} + \frac{8}{10}} = y^{\frac{10}{10}} = y^1 = y$
2. $\frac{\sqrt{a} \cdot \sqrt[3]{a} \cdot \sqrt[4]{a} }{\sqrt[12]{a}} = \frac{a^{\frac{1}{2}} \cdot a^{\frac{1}{3}} \cdot a^{\frac{1}{4}}}{a^{\frac{1}{12}}} = \frac{a^{\frac{1 \cdot 6}{2 \cdot 6}} \cdot a^{\frac{1 \cdot 4}{3 \cdot 4}} \cdot a^{\frac{1 \cdot 3}{4 \cdot 3}}}{a^{\frac{1}{12}}} = \frac{a^{\frac{6}{12}} \cdot a^{\frac{4}{12}} \cdot a^{\frac{3}{12}}}{a^{\frac{1}{12}}} = a^{\frac{6}{12} + \frac{4}{12} + \frac{3}{12} - \frac{1}{12}} = a^{\frac{12}{12} = a^1 = a}$
3. $\sqrt[4]{25^5} \cdot 25^{-\frac{3}{4}} = 25^{\frac{5}{4}} \cdot 25^{-\frac{3}{4}} = 25^{\frac{5}{4} - \frac{3}{4}} = 25^{\frac{2}{4}} = 25^{\frac{1}{2}} = \sqrt{25} = 5$
4. $a \cdot \sqrt[3]{a^5} \cdot a^{- \frac{2}{3}} = a \cdot a^{\frac{5}{3}} \cdot a^{-\frac{2}{3}} = a^{\frac{5}{3} + \frac{3}{3} - \frac{2}{3}} = a^{\frac{6}{3}} = a^2$
